\documentclass[10pt,a4paper]{article}
\usepackage[natbibapa]{apacite} 
\usepackage{amsmath}
\usepackage{textcomp}
\usepackage[a4paper,margin=0.8in]{geometry} 

%opening
\title{COS 4807 Assignment 1}
\author{Adriaan Louw (53031377)}

\begin{document}

\maketitle

\section{Question 1.1}

\begin{tabular}{|c|c|c|c|c|c|c|c|c|c|}
\hline
$p$ & $q$ & $r$ & $\neg p$ & $ \neg q$ & $p \vee q$ & $(p \vee q) \vee r$ & $\neg p \wedge \neg q$ &  $((( p \vee q) \vee r ) \wedge ( \neg p \wedge \neg q ))$ & $ ((( p \vee q) \vee r ) \wedge ( \neg p \wedge \neg q )) \rightarrow r$\\ 
\hline
 0 &  0 & 0 & 1 & 1 & 0 & 0 & 1 & 0 & 1\\
 0 &  0 & 1 & 1 & 1 & 0 & 1 & 1 & 1 & 1\\
 0 &  1 & 0 & 1 & 0 & 1 & 1 & 0 & 0 & 1\\
 0 &  1 & 1 & 1 & 0 & 1 & 1 & 0 & 0 & 1\\
 1 &  0 & 0 & 0 & 1 & 1 & 1 & 0 & 0 & 1\\
 1 &  0 & 1 & 0 & 1 & 1 & 1 & 0 & 0 & 1\\
 1 &  1 & 0 & 0 & 0 & 1 & 1 & 0 & 0 & 1\\
 1 &  1 & 1 & 0 & 0 & 1 & 1 & 0 & 0 & 1\\
\hline
\end{tabular}


\section{Question1.2}

\begin{tabular}{|c|c|c|}
\hline
$p$ & $q$ & $r$ \\ 
\hline
 0 &  0 & 0 \\
 0 &  0 & 1 \\
 0 &  1 & 0 \\
 0 &  1 & 1 \\
 1 &  0 & 0 \\
 1 &  0 & 1 \\
 1 &  1 & 0 \\
 1 &  1 & 1 \\
\hline
\end{tabular}



\section{Question 4.1}
For formula

\begin{equation}
\label{41}
 ((( p \vee q) \vee r ) \wedge ( \neg p \wedge \neg q )) \rightarrow r
\end{equation}

Applying the $\beta$ formula for implication gives

\begin{equation}
\label{411}
 \neg  ((( p \vee q) \vee r ) \wedge ( \neg p \wedge \neg q ))
\end{equation}

and

\begin{equation}
\label{412}
 r
\end{equation}

Where Formula \ref{412} is satisfyable.

Continueing for Formula \ref{411} by applying the $\beta$ formula for $\neg (B_1 \wedge B_2)$ we get



 \begin{equation}
 \label{4111}
  \neg (( p \vee q ) \vee r )
 \end{equation}

 and 
 
 \begin{equation}
 \label{4112}
  \neg ( \neg p \wedge \neg q )
 \end{equation}


Continueing for Formula \ref{4111} and applying $\alpha$ formula $\neg ( A_1 \vee A_2 )$ we get

\begin{equation}
\label{41111}
 \neg (p \vee q), \neg r 
\end{equation}

Then applying formula $\neg ( A_1 \vee A_2 )$ again we get

\begin{equation}
\label{411111}
 \neg p, \neg q, \neg r
\end{equation}

Which is satisfyable.

Going back to Formula \ref{4112} which can by simplified to 

\begin{equation}
 p \vee q
\end{equation}

Then applying $\beta$ formula $B_1 \vee B_2$ we get formulas

\begin{equation}
 \label{41121}
 p
\end{equation}

and 

\begin{equation}
\label{41122}
q
\end{equation}

Both of which are satifyable. Now looking at all the leaf nodes namely 
Formalas \ref{412}, \ref{411111}, \ref{41121} and \ref{41122} we can see that they are all satisfyable. Thus
Formula \ref{41} is valid.







\section{Question 4.2}

\begin{equation}
\label{420}
(p \rightarrow ( q \rightarrow r )) \leftrightarrow (( p \wedge q) \wedge \neg r) 
\end{equation}

By substituting for double implication operator:

\begin{equation}
 (p \rightarrow ( q \rightarrow r )) \rightarrow (( p \wedge q) \wedge \neg r), (( p \wedge q) \wedge \neg r) \rightarrow (p \rightarrow ( q \rightarrow r )) 
\end{equation}

Substituting for the implication operator in the first term gives:

\begin{equation}
\label{421}
 \neg(p \rightarrow ( q \rightarrow r )),  (( p \wedge q) \wedge \neg r) \rightarrow (p \rightarrow ( q \rightarrow r )) 
\end{equation}

and

\begin{equation}
\label{422}
 ((p \wedge q) \wedge \neg r ),  (( p \wedge q) \wedge \neg r) \rightarrow (p \rightarrow ( q \rightarrow r )) 
\end{equation}

Equation \ref{421} becomes

\begin{equation}
p, \neg ( q \rightarrow r )),  (( p \wedge q) \wedge \neg r) \rightarrow (p \rightarrow ( q \rightarrow r )) 
\end{equation}

then 

\begin{equation}
\label{421a}
p, q, \neg r, (( p \wedge q) \wedge \neg r) \rightarrow (p \rightarrow ( q \rightarrow r )) 
\end{equation}

Substituting for the implication in the above formula gives:

\begin{equation}
\label{4211}
p, q, \neg r, \neg (( p \wedge q) \wedge \neg r)
\end{equation}

and

\begin{equation}
\label{4212}
p, q, \neg r, (p \rightarrow ( q \rightarrow r )) 
\end{equation}


Formula \ref{4211} becomes 


\begin{equation}
\label{42111}
p, q, \neg r, \neg ( p \wedge q)
\end{equation}

and 

\begin{equation}
\label{42112}
p, q, \neg r, r
\end{equation}

We can see that Formula \ref{42112} is unsatifyable.  Then Formula \ref{42111} becomes

\begin{equation}
\label{421111}
p, q, \neg r, \neg p 
\end{equation}

and 

\begin{equation}
\label{421112}
p, q, \neg r, \neg q 
\end{equation}

Both of which are unsatifyable. Now having done all the leaves under Formula \ref{4211}, we continue with the leaves under Equation \ref{4212}.

Equation \ref{4212} becomes

\begin{equation}
\label{42121}
p, q, \neg r, \neg p 
\end{equation}

which is unsatifyable and
 
\begin{equation}
\label{42122}
p, q, \neg r, q \rightarrow r 
\end{equation} 

which becomes

\begin{equation}
\label{421221}
p, q, \neg r, \neg q,  r 
\end{equation} 
 
Having finished all the leaves under Formula \ref{421} we continue with Formula \ref{422} which becomes

\begin{equation}
\label{4221}
 p, q, \neg r,  (( p \wedge q) \wedge \neg r) \rightarrow (p \rightarrow ( q \rightarrow r )) 
\end{equation} 

But Formula \ref{4221} is the same as Formula \ref{421a}. Formula \ref{421a} will have the same leaf nodes as Formula \ref{4221}.

Thus we have all the leaf nodes namely Formulas \ref{42112}, \ref{421111}, \ref{421112}, \ref{42121} and \ref{421221}. All of these Formulas are unsatisfyable, 
therefore the original Formula \ref{420} is unsatisfyable.

\end{document}
