\documentclass[10pt,a4paper]{article}
\usepackage[natbibapa]{apacite} 
\usepackage{amsmath}
\usepackage{textcomp}
\usepackage[a4paper,margin=0.8in]{geometry} 
\usepackage{latexsym}
\usepackage{tikz}
\usepackage{etoolbox}
\usepackage{mathrsfs}

%opening
\title{COS 4807 Assignment 4}
\author{Adriaan Louw (53031377)}

\newcommand{\interp}{\mathscr{I}}


\tikzset{
  treenode/.style = {shape=rectangle, rounded corners,
                     draw, align=center,
                     top color=white, bottom color=blue!20},
  root/.style     = {treenode, font=\Large, bottom color=red!30},
  env/.style      = {treenode, font=\ttfamily\normalsize},
  dummy/.style    = {circle,draw}
}

\usetikzlibrary{shapes.misc}


\begin{document}

\maketitle


\section{Question 1i}

\begin{equation}
 \exists x p(x)\rightarrow \exists y(p(y)\wedge\exists x q(x,y))
\end{equation}

\begin{equation}
 \exists x p(x)\rightarrow \exists y(p(y)\wedge\exists z q(z,y))
\end{equation}

Using $A\rightarrow B \equiv \neg A \vee B$

\begin{equation}
 \neg\exists x p(x)\rightarrow \exists y(p(y)\wedge\exists z q(z,y))
\end{equation}

\begin{equation}
 \forall x \neg p(x)\rightarrow \exists y(p(y)\wedge\exists z q(z,y))
\end{equation}

\begin{equation}
 \forall x (\neg p(x)\rightarrow \exists y(p(y)\wedge\exists z q(z,y)))
\end{equation}

\begin{equation}
 \forall x\exists y (\neg p(x)\rightarrow (p(y)\wedge\exists z q(z,y)))
\end{equation}

\begin{equation}
 \forall x\exists y \exists z (\neg p(x)\rightarrow (p(y)\wedge q(z,y)))
\end{equation}

Using distributivity of $\vee$ and $\wedge$

\begin{equation}
 \forall x\exists y \exists z ((\neg p(x) \vee p(y))\wedge(\neg (p(x) \vee q(z,y))))
\end{equation}

\begin{equation}
 \forall x\exists y ((\neg p(x) \vee p(y))\wedge(\neg (p(x) \vee q(f(x),y))))
\end{equation}


\begin{equation}
 \forall x ((\neg p(x) \vee p(g(x)))\wedge(\neg (p(x) \vee q(f(x),g(x)))))
\end{equation}

\begin{equation}
 \{\{\neg p(x),p(g(x))\},\{\neg p(x),q(f(x),g(x))\}\}
\end{equation}



\section{Question 1ii}

\begin{equation}
 \forall x ((\forall y q(x,y) \vee \forall z q(z,x))\rightarrow g(x,x))
\end{equation}

Using $A\rightarrow B \equiv \neg A \vee B$

\begin{equation}
 \forall x (\neg(\forall y q(x,y) \vee \forall z q(z,x))\vee g(x,x))
\end{equation}


\begin{equation}
 \forall x ((\neg\forall y q(x,y) \wedge \neg \forall z q(z,x))\vee g(x,x))
\end{equation}

\begin{equation}
 \forall x (( \exists y \neg q(x,y) \wedge  \exists z \neg q(z,x))\vee g(x,x))
\end{equation}

\begin{equation}
 \forall x \exists y((  \neg q(x,y) \wedge  \exists z \neg q(z,x))\vee g(x,x))
\end{equation}
\begin{equation}
 \forall x \exists y\exists z((  \neg q(x,y) \wedge   \neg q(z,x))\vee g(x,x))
\end{equation}


Using distributivity of $\vee$ and $\wedge$


\begin{equation}
 \forall x \exists y\exists z(( q(x,x) \vee \neg q(x,y))\wedge (q(x,x) \vee \neg q(z,x)))
\end{equation}


\begin{equation}
 \forall x \exists y(( q(x,x) \vee \neg q(x,y))\wedge (q(x,x) \vee \neg q(f(x),x)))
\end{equation}

\begin{equation}
 \forall x (( q(x,x) \vee \neg q(x,g(x)))\wedge (q(x,x) \vee \neg q(f(x),x)))
\end{equation}


\begin{equation}
 \{\{q(x,x),\neg q(x,g(x))\},\{q(x,x),q(f(x),x)\}\}
\end{equation}



\section{Question 1ii}


\begin{equation}
 \forall x \forall y(\exists z p(z) \leftrightarrow q(x,y))
\end{equation}

Using $A\leftrightarrow B \equiv (A\rightarrow B)\wedge (B\rightarrow A)$

\begin{equation}
 \forall x \forall y((\exists z p(z) \rightarrow q(x,y))\wedge(q(x,y)\rightarrow \exists z p(z)))
\end{equation}

\begin{equation}
 \forall x \forall y((\exists z p(z) \rightarrow q(x,y))\wedge(q(x,y)\rightarrow \exists k p(k)))
\end{equation}


Using $A\rightarrow B \equiv \neg A \vee B$


\begin{equation}
 \forall x \forall y((\neg\exists z p(z) \vee q(x,y))\wedge(\neg q(x,y) \vee \exists k p(k)))
\end{equation}

\begin{equation}
 \forall x \forall y(( \forall z \neg p(z) \vee q(x,y))\wedge(\neg q(x,y) \vee \exists k p(k)))
\end{equation}

\begin{equation}
 \forall x \forall y \forall z \exists k(( \neg p(z) \vee q(x,y))\wedge(\neg q(x,y) \vee p(k)))
\end{equation}

\begin{equation}
 \forall x \forall y \forall z (( \neg p(z) \vee q(x,y))\wedge(\neg q(x,y) \vee p(f(x,y,z))))
\end{equation}


\begin{equation}
 \{\{\neg p(z),q(x,y)\},\{\neg q(x,y),p(f(x,y,z)\}\}
\end{equation}


\end{document}
